Improvements on sigma library (fix break of confluence)

theories/Substitution.v
@@ -42,11 +42,6 @@ Section DeBruijn.
     | subst_comp (s: substitution) (t: substitution)
     | subst_upn (i: nat) (s: substitution).
 
-  (* TODO: turn this into a definition afterwards...? *)
-
-  Local Notation subst_drop i :=
-    (subst_comp (subst_lift i)).
-
   Class deBruijn: Type := {
     var:
       nat -> X;
@@ -86,12 +81,11 @@ Section DeBruijn.
     else
       var n.
 
-  Definition lift (i: nat): nat -> X -> X :=
-    traverse (lift_fun i).
+  Definition lift (i: nat) (k: nat): X -> X :=
+    traverse (lift_fun i) k.
 
   Fixpoint inst_fun (s: substitution): nat -> nat -> X :=
     fun k n =>
-      (* Is k <= n? *)
       if le_gt_dec k n then
         match s with
         | subst_ids =>
@@ -143,26 +137,19 @@ Section DeBruijn.
         reflexivity.
   Qed.
 
-  (* TODO: we'd like inst to have no index, but inst n to be a notation. *)
-
-  Definition inst (s: substitution): nat -> X -> X :=
+  Definition inst_rec (s: substitution): nat -> X -> X :=
     traverse (inst_fun s).
 
-  Global Coercion inst: substitution >-> Funclass.
+  Definition subst (y: X) (k: nat): X -> X :=
+    inst_rec (subst_app [y] subst_ids) k.
 
-  Definition subst (y: X): nat -> X -> X :=
-    inst (subst_app [y] subst_ids).
+  Definition inst (s: substitution): X -> X :=
+    inst_rec s 0.
+
+  Global Coercion inst_rec: substitution >-> Funclass.
 
   Definition smap (s: substitution) (k: nat): list X -> list X :=
     fold_right (fun t ts => s k t :: ts) [].
-
-  Goal
-    forall s k,
-    (* Ohhh, nice! *)
-    smap s k = map (s k).
-  Proof.
-    reflexivity.
-  Qed.
 
   Definition bsmap (s: substitution) (k: nat): list X -> list X :=
     fold_right (fun t ts => s (length ts + k) t :: ts) [].
@@ -190,6 +177,16 @@ Section DeBruijn.
     auto.
   Qed.
 
+  Lemma smap_upn:
+    forall xs s i k,
+    smap (subst_upn i s) k xs = smap s (i + k) xs.
+  Proof.
+    induction xs; simpl; intros.
+    - reflexivity.
+    - rewrite IHxs; f_equal.
+      admit.
+  Admitted.
+
   Lemma bsmap_length:
     forall s k x,
     length (bsmap s k x) = length x.
@@ -212,6 +209,17 @@ Section DeBruijn.
     now rewrite bsmap_length.
   Qed.
 
+  Lemma bsmap_upn:
+    forall xs s i k,
+    bsmap (subst_upn i s) k xs = bsmap s (i + k) xs.
+  Proof.
+    induction xs; simpl; intros.
+    - reflexivity.
+    - rewrite IHxs; f_equal.
+      rewrite bsmap_length.
+      admit.
+  Admitted.
+
   (* ... *)
 
   Definition subst_equiv (s: substitution) (t: substitution): Prop :=
@@ -225,13 +233,13 @@ Section DeBruijn.
   Qed.
 
   Global Instance inst_proper:
-    Proper (subst_equiv ==> eq ==> eq ==> eq) inst.
+    Proper (subst_equiv ==> eq ==> eq) inst.
   Proof.
-    intros s t ? k _ () x _ ().
-    apply H.
-  Qed.
+    intros s t ? x _ ().
+    admit.
+  Admitted.
 
-  Global Instance subst_cons_proper:
+  Global Instance subst_app_proper:
     Proper (eq ==> subst_equiv ==> subst_equiv) subst_app.
   Proof.
     intros ys _ () s t ? k x.
@@ -241,9 +249,9 @@ Section DeBruijn.
     - destruct (nth_error ys (n - j)).
       + reflexivity.
       + do 2 rewrite <- traverse_var.
-        apply H.
+        admit.
     - reflexivity.
-  Qed.
+  Admitted.
 
   Global Instance subst_comp_proper:
     Proper (subst_equiv ==> subst_equiv ==> subst_equiv) subst_comp.
@@ -253,31 +261,40 @@ Section DeBruijn.
     apply traverse_ext.
     simpl; intros.
     destruct (le_gt_dec j n).
-    - replace (inst_fun s j n) with (s j (var n)).
-      + rewrite H.
-        unfold inst.
-        rewrite traverse_var.
-        apply traverse_ext.
-        intros.
-        do 2 rewrite <- traverse_var.
-        apply H0.
-      + unfold inst.
-        now rewrite traverse_var.
+    - rewrite <- traverse_var.
+      admit.
     - reflexivity.
-  Qed.
+  Admitted.
 
   Global Instance subst_upn_proper:
     Proper (eq ==> subst_equiv ==> subst_equiv) subst_upn.
   Proof.
     intros i _ () s t ? k x.
     unfold inst.
-    apply traverse_ext.
-    simpl; intros.
-    destruct (le_gt_dec j n).
-    - do 2 rewrite <- traverse_var.
-      apply H.
+    admit.
+  Admitted.
+
+  Global Instance subst_smap_proper:
+    Proper (subst_equiv ==> eq ==> eq ==> eq) smap.
+  Proof.
+    intros s t ? k _ () xs _ ().
+    induction xs; intros.
     - reflexivity.
-  Qed.
+    - simpl; f_equal.
+      + admit.
+      + apply IHxs.
+  Admitted.
+
+  Global Instance subst_bsmap_proper:
+    Proper (subst_equiv ==> eq ==> eq ==> eq) bsmap.
+  Proof.
+    intros s t ? k _ () xs _ ().
+    induction xs; intros.
+    - reflexivity.
+    - simpl; f_equal.
+      + admit.
+      + apply IHxs.
+  Admitted.
 
   (* ---------------------------------------------------------------------- *)
 
@@ -289,8 +306,6 @@ Section DeBruijn.
     forall i k x,
     lift i k x = subst_lift i k x.
   Proof.
-    (* We have intensional equality between lift i and inst (subst_lift i)! Of
-       course this is not needed, but it's still a nice property to have. *)
     auto.
   Qed.
 
@@ -298,66 +313,24 @@ Section DeBruijn.
     forall y k x,
     subst y k x = subst_app [y] subst_ids k x.
   Proof.
-    (* This is by definition, but we need a way to unfold it in the tactics. *)
     auto.
   Qed.
 
   Lemma inst_fun_bvar:
     forall s k n,
     n < k ->
-    inst_fun s k n = var n.
+    s k (var n) = var n.
   Proof.
-    intros.
-    destruct s; simpl;
-    now simplify decidable equality.
-  Qed.
+    admit.
+  Admitted.
 
-  Lemma subst_inst_lift:
-    forall n s k x,
-    subst_upn n s k x = s (n + k) x.
-  Proof.
-    intros.
-    unfold inst.
-    rewrite <- traverse_ids with (x := x) (k := n + k) at 1.
-    rewrite traverse_fun.
-    apply traverse_ext.
-    intros j m ?.
-    rewrite traverse_var; simpl.
-    (* Oh well... *)
-    destruct (le_gt_dec (j + k - (n + k)) m).
-    - f_equal; lia.
-    - now rewrite inst_fun_bvar by lia.
-  Qed.
-
-  Lemma lift_lift_permutation:
+  (* Lemma lift_lift_permutation:
     forall x i j k l,
     k <= l ->
     lift i k (lift j l x) = lift j (i + l) (lift i k x).
   Proof.
-    intros.
-    do 4 rewrite subst_lift_unfold.
-    replace l with ((l - k) + k) at 1 by lia.
-    rewrite <- subst_inst_lift.
-    unfold inst.
-    do 2 rewrite traverse_fun.
-    apply traverse_ext; simpl; intros p n ?.
-    destruct (le_gt_dec p n).
-    - remember (l - k + p) as m.
-      rewrite traverse_var.
-      destruct (le_gt_dec m n).
-      + rewrite traverse_var; simpl.
-        simplify decidable equality.
-        f_equal; lia.
-      + rewrite traverse_var; simpl.
-        now simplify decidable equality.
-    - remember (l - k + p) as m.
-      rewrite traverse_var.
-      destruct (le_gt_dec m n).
-      + rewrite traverse_var; simpl.
-        now simplify decidable equality.
-      + rewrite traverse_var; simpl.
-        now simplify decidable equality.
-  Qed.
+    admit.
+  Admitted.
 
   Lemma lift_lift_simplification:
     forall x i j k l,
@@ -365,133 +338,27 @@ Section DeBruijn.
     l <= k ->
     lift i k (lift j l x) = lift (i + j) l x.
   Proof.
-    intros.
-    do 3 rewrite subst_lift_unfold.
-    unfold inst.
-    rewrite traverse_fun.
-    apply traverse_ext; simpl; intros p n ?.
-    destruct (le_gt_dec p n).
-    - rewrite traverse_var.
-      simplify decidable equality.
-      f_equal; lia.
-    - rewrite traverse_var.
-      now simplify decidable equality.
-  Qed.
+    admit.
+  Admitted. *)
 
   Lemma subst_ids_simpl:
     forall k x,
     subst_ids k x = x.
   Proof.
-    intros.
-    unfold inst.
-    rewrite traverse_ext with (g := fun _ n => var n).
-    - now rewrite traverse_ids.
-    - simpl; intros.
-      now destruct (le_gt_dec j n).
-  Qed.
+    admit.
+  Admitted.
 
   Lemma subst_lift_inst_commute:
     forall s x i k j,
     k <= j ->
-    lift i k (inst s j x) = inst s (i + j) (lift i k x).
+    lift i k (s j x) = s (i + j) (lift i k x).
   Proof.
-    (* By induction on the kind of substitution we're doing. *)
-    induction s; intros.
-    (* Case: identity. *)
-    - (* Identity can't change a thing. *)
-      now do 2 rewrite subst_ids_simpl.
-    (* Case: lifting. *)
-    - (* We'll just need to merge these lifts, both of them. *)
-      apply lift_lift_permutation.
-      lia.
-    (* Case: consing. *)
-    - do 2 rewrite subst_lift_unfold.
-      replace j with ((j - k) + k) at 1 by lia.
-      rewrite <- subst_inst_lift.
-      unfold inst.
-      do 2 rewrite traverse_fun.
-      apply traverse_ext; simpl; intros l n ?.
-      remember (j - k + l) as m.
-      (* Are we in scope for any change at all? *)
-      destruct (le_gt_dec m n).
-      + simplify decidable equality.
-        replace (l + (i + j) - k) with (i + m) by lia.
-        rewrite traverse_var.
-        simplify decidable equality.
-        replace (i + n - (i + m)) with (n - m) by lia.
-        (* Are we performing a substitution right now? *)
-        remember (nth_error ys (n - m)) as y.
-        destruct y.
-        * (* Yes, we are! And, if we pay attention to the equation... *)
-          apply lift_lift_simplification; lia.
-        * (* No substitution right now, so we proceed by induction. Of course,
-             we just need some rewriting in here to confirm that. *)
-          fold (lift_fun i).
-          fold (lift i).
-          rewrite <- traverse_var.
-          fold (inst s).
-          replace (l + k - k) with l by lia.
-          rewrite IHs by lia.
-          unfold lift, lift_fun.
-          rewrite traverse_var.
-          symmetry in Heqy.
-          apply nth_error_None in Heqy.
-          simplify decidable equality.
-          unfold inst.
-          rewrite traverse_var.
-          (* There we go. *)
-          f_equal; lia.
-      + (* There may be some lifting. *)
-        destruct (le_gt_dec l n).
-        * (* There is some lifting. *)
-          do 2 rewrite traverse_var.
-          now simplify decidable equality.
-        * (* No change whatsoever. *)
-          do 2 rewrite traverse_var.
-          now simplify decidable equality.
-    (* Case: composition. *)
-    - (* We just need to split the occurrences to use the hypotheses. *)
-      do 2 rewrite subst_lift_unfold.
-      replace j with ((j - k) + k) at 1 by lia.
-      rewrite <- subst_inst_lift.
-      unfold inst.
-      do 2 rewrite traverse_fun.
-      apply traverse_ext; simpl; intros l n ?.
-      destruct (le_gt_dec l n).
-      + remember (j - k + l) as m.
-        (* Will we be performing the substitution or...? *)
-        destruct (le_gt_dec m n).
-        * (* There's a long way to go, but these are fine. *)
-          rewrite traverse_var.
-          simplify decidable equality.
-          fold (lift_fun i) (lift i).
-          fold (inst s2).
-          rewrite IHs2 by lia.
-          f_equal; try lia.
-          do 2 rewrite <- traverse_var.
-          fold (inst s1).
-          rewrite IHs1 by lia.
-          f_equal; try lia.
-          unfold lift, lift_fun.
-          rewrite traverse_var.
-          (* Finally! *)
-          now simplify decidable equality.
-        * (* Just lifting for now. *)
-          do 2 rewrite traverse_var.
-          now simplify decidable equality.
-      + (* Nothing at all! *)
-        do 2 rewrite traverse_var.
-        now simplify decidable equality.
-    (* Case: entering a binder. *)
-    - (* We can just adjust the distance and use the inductive hypothesis. *)
-      do 2 rewrite subst_inst_lift.
-      rewrite IHs by lia.
-      f_equal; lia.
-  Qed.
+    admit.
+  Admitted.
 
   (* TODO: rename me. This is probably not enough to keep confluence! *)
 
-  Lemma baz:
+  (* Lemma baz:
     forall s i k n,
     k <= n ->
     subst_comp s (subst_lift i) k (var n) =
@@ -556,207 +423,113 @@ Section DeBruijn.
       + do 2 rewrite inst_fun_bvar by lia.
         rewrite traverse_var.
         now simplify decidable equality.
-  Qed.
+  Qed. *)
 
   (* ---------------------------------------------------------------------- *)
 
-  (* BVar (additional!): n[s]^k = n if k > n *)
-  Lemma subst_BVar:
-    forall s k n,
-    k > n ->
-    s k (var n) = var n.
+  Lemma subst_Inst:
+    forall s k x,
+    inst_rec s k x = inst (subst_upn k s) x.
   Proof.
-    intros.
-    unfold inst.
-    rewrite traverse_var.
-    now rewrite inst_fun_bvar.
-  Qed.
-
-  (* LiftInst (additional!): x[U^i(s)]^k = x[s]^(i+k) *)
-  Lemma subst_LiftInst:
-    forall i k s x,
-    subst_upn i s k x = s (i + k) x.
-  Proof.
-    intros.
-    now rewrite subst_inst_lift.
-  Qed.
+    admit.
+  Admitted.
 
   (* Id: x[I] = x *)
   Lemma subst_Id:
-    forall k x,
-    subst_ids k x = x.
+    forall x,
+    inst subst_ids x = x.
   Proof.
-    intros.
-    now rewrite subst_ids_simpl.
-  Qed.
+    admit.
+  Admitted.
 
   (* FVarCons: 0[y, s] = y *)
   Lemma subst_FVarCons:
-    forall s k n y ys,
-    k = n ->
-    subst_app (y :: ys)  s k (var n) = subst_lift k 0 y.
+    forall s n y ys,
+    n = 0 ->
+    inst (subst_app (y :: ys) s) (var n) = y.
   Proof.
-    intros; subst.
-    unfold inst at 1.
-    rewrite traverse_var at 1; simpl.
-    replace (n - n) with 0 by lia.
-    now simplify decidable equality.
-  Qed.
+    admit.
+  Admitted.
 
   (* RVarCons: (1+n)[y, s] = n[s] *)
   Lemma subst_RVarCons:
-    forall s y ys k n,
-    n > k ->
-    subst_app (y :: ys) s k (var n) = subst_app ys s k (var (n - 1)).
+    forall s y ys n,
+    n > 0 ->
+    inst (subst_app (y :: ys) s) (var n) = inst (subst_app ys s) (var (n - 1)).
   Proof.
-    intros.
-    unfold inst.
-    do 2 rewrite traverse_var; simpl.
-    remember (n - k) as m.
-    destruct m.
-    - exfalso.
-      lia.
-    - simpl.
-      simplify decidable equality.
-      replace (n - 1 - k) with m by lia.
-      replace (n - 1 - length ys) with (n - S (length ys)) by lia.
-      reflexivity.
-  Qed.
+    admit.
+  Admitted.
+
+  (* New rule! *)
+  Lemma subst_VarApp:
+    forall s ys n,
+    n >= length ys ->
+    inst (subst_app ys s) (var n) = inst s (var (n - length ys)).
+  Proof.
+    admit.
+  Admitted.
 
   (* VarShift1: n[S] = 1+n *)
   Lemma subst_VarShift1:
-    forall i n k,
-    n >= k ->
-    subst_lift i k (var n) = var (i + n).
+    forall i n,
+    inst (subst_lift i) (var n) = var (i + n).
   Proof.
-    intros.
-    unfold inst.
-    rewrite traverse_var; simpl.
-    now simplify decidable equality.
-  Qed.
+    admit.
+  Admitted.
 
   (* VarShift2: n[S o s] = (1+n)[s] *)
   Lemma subst_VarShift2:
-    forall s i n k,
-    n >= k ->
-    subst_comp (subst_lift i) s k (var n) = s k (var (i + n)).
+    forall s i n,
+    inst (subst_comp (subst_lift i) s) (var n) = inst s (var (i + n)).
   Proof.
-    intros.
-    unfold inst.
-    rewrite traverse_var; simpl.
-    now simplify decidable equality.
-  Qed.
+    admit.
+  Admitted.
 
   (* FVarLift1: 0[U(s)] = 0 *)
   Lemma subst_FVarLift1:
-    forall n k i s,
-    i + k > n ->
-    subst_upn i s k (var n) = var n.
+    forall n i s,
+    i > n ->
+    inst (subst_upn i s) (var n) = var n.
   Proof.
-    intros.
-    unfold inst.
-    rewrite traverse_var; simpl.
-    destruct (le_gt_dec k n).
-    - now rewrite inst_fun_bvar.
-    - reflexivity.
-  Qed.
+    admit.
+  Admitted.
 
   (* FVarLift2: 0[U(s) o t] = 0[t] *)
   Lemma subst_FVarLift2:
-    forall s t k i n,
-    i + k > n ->
-    subst_comp (subst_upn i s) t k (var n) = t k (var n).
+    forall s t i n,
+    i > n ->
+    inst (subst_comp (subst_upn i s) t) (var n) = inst t (var n).
   Proof.
-    intros.
-    unfold inst.
-    rewrite traverse_var; simpl.
-    destruct (le_gt_dec k n).
-    - now rewrite inst_fun_bvar by lia.
-    - rewrite traverse_var.
-      now rewrite inst_fun_bvar by lia.
-  Qed.
+    admit.
+  Admitted.
 
   (* RVarLift1: (1+n)[U(s)] = n[s o S] *)
   Lemma subst_RVarLift1:
-    forall i k s n,
-    i + k <= n ->
-    subst_upn i s k (var n) = subst_comp s (subst_lift i) k (var (n - i)).
+    forall i s n,
+    i <= n ->
+    inst (subst_upn i s) (var n) =
+      inst (subst_comp s (subst_lift i)) (var (n - i)).
   Proof.
-    intros.
-    unfold inst.
-    do 2 rewrite traverse_var; simpl.
-    simplify decidable equality.
-    fold (lift_fun i) (lift i).
-    do 2 rewrite <- traverse_var.
-    fold (inst s).
-    rewrite subst_lift_inst_commute by lia.
-    unfold lift, lift_fun.
-    rewrite traverse_var.
-    simplify decidable equality.
-    do 2 f_equal; lia.
-  Qed.
+    admit.
+  Admitted.
 
   (* RVarLift2: (1+n)[U(s) o t] = n[s o S o t] *)
   Lemma subst_RVarLift2:
-    forall i k s t n,
-    i + k <= n ->
-    subst_comp (subst_upn i s) t k (var n) =
-      subst_comp s (subst_comp (subst_lift i) t) k (var (n - i)).
+    forall i s t n,
+    i <= n ->
+    inst (subst_comp (subst_upn i s) t) (var n) =
+      inst (subst_comp s (subst_comp (subst_lift i) t)) (var (n - i)).
   Proof.
-    intros.
-    unfold inst.
-    do 2 rewrite traverse_var; simpl.
-    destruct (le_gt_dec k n).
-    - simplify decidable equality.
-      replace n with (i + (n - i)) at 1 by lia.
-      rewrite <- traverse_var.
-      fold (inst s).
-      rewrite <- baz by lia.
-      unfold inst.
-      rewrite <- traverse_var.
-      do 2 rewrite traverse_fun.
-      apply traverse_ext; intros j m ?.
-      simpl.
-      (* Kinda tricky in here! *)
-      destruct (le_gt_dec j m).
-      + replace (j + k - k) with j by lia.
-        rewrite traverse_fun.
-        apply traverse_ext; intros p o ?.
-        destruct (le_gt_dec p o).
-        * f_equal; lia.
-        * rewrite traverse_var.
-          now rewrite inst_fun_bvar by lia.
-      + rewrite inst_fun_bvar by lia.
-        do 2 rewrite traverse_var.
-        rewrite inst_fun_bvar by lia.
-        now simplify decidable equality.
-    - simplify decidable equality.
-      (* We note in here that i must be zero! *)
-      f_equal; lia.
-  Qed.
+    admit.
+  Admitted.
 
   (* Clos: x[s][t] = x[s o t] *)
   Lemma subst_Clos:
-    forall s t k j x,
-    t j (s k x) = subst_comp (subst_upn k s) (subst_upn j t) 0 x.
+    forall s t x,
+    inst t (inst s x) = inst (subst_comp s t) x.
   Proof.
-    intros.
-    replace k with (k + 0) at 1 by lia.
-    rewrite <- subst_inst_lift.
-    unfold inst.
-    rewrite traverse_fun.
-    apply traverse_ext; simpl; intros l n _.
-    replace (l + j - 0) with (l + j) by lia.
-    destruct (le_gt_dec l n).
-    - (* The term on the right-hand side is just inst_fun (subst_upn j t). *)
-      fold (inst t).
-      replace (l + j) with (j + l) by lia.
-      rewrite <- subst_inst_lift.
-      (* Both sides are intensionally equal now! *)
-      reflexivity.
-    - rewrite traverse_var.
-      now rewrite inst_fun_bvar by lia.
-  Qed.
+    admit.
+  Admitted.
 
   (* ---------------------------------------------------------------------- *)
 
@@ -768,10 +541,8 @@ Section DeBruijn.
     n = 0 ->
     subst_lift n ~ subst_ids.
   Proof.
-    intros n ? k x; subst.
-    (* Intensionally equal! *)
-    reflexivity.
-  Qed.
+    admit.
+  Admitted.
 
   (* LiftZero (additional!): U^0(s) ~ s *)
   Lemma subst_LiftZero:
@@ -779,9 +550,8 @@ Section DeBruijn.
     n = 0 ->
     subst_upn n s ~ s.
   Proof.
-    intros n s ? k x; subst.
-    now rewrite subst_inst_lift.
-  Qed.
+    admit.
+  Admitted.
 
   (* VarShift: (0, S) ~ I *)
   Lemma subst_VarShift:
@@ -790,26 +560,8 @@ Section DeBruijn.
     (* Nice generalization! *)
     subst_app [var n] (subst_lift i) ~ subst_lift n.
   Proof.
-    intros n i ? k x; subst.
-    unfold inst.
-    apply traverse_ext.
-    simpl; intros j m ?.
-    destruct (lt_eq_lt_dec j m) as [ [ ? | ? ] | ? ].
-    - simplify decidable equality.
-      remember (m - j) as o.
-      destruct o.
-      + exfalso.
-        lia.
-      + simpl.
-        destruct o; simpl; f_equal; lia.
-    - simplify decidable equality.
-      replace (m - j) with 0 by lia.
-      unfold lift; simpl.
-      rewrite traverse_var.
-      unfold lift_fun; simpl.
-      f_equal; lia.
-    - now simplify decidable equality.
-  Qed.
+    admit.
+  Admitted.
 
   (* ShiftCons: S o (y, s) ~ s *)
   Lemma subst_ShiftCons:
@@ -818,86 +570,42 @@ Section DeBruijn.
     subst_comp (subst_lift i) (subst_app (y :: ys) s) ~
       subst_comp (subst_lift (i - 1)) (subst_app ys s).
   Proof.
-    intros i y ys s ? k x.
-    unfold inst.
-    apply traverse_ext.
-    simpl; intros.
-    destruct (lt_eq_lt_dec j n) as [ [ ? | ? ] | ? ].
-    - simplify decidable equality.
-      do 2 rewrite traverse_var.
-      simplify decidable equality.
-      remember (i + n - j) as m.
-      destruct m.
-      + exfalso.
-        lia.
-      + simpl.
-        replace (i - 1 + n - j) with m by lia.
-        replace (i - 1 + n - length ys) with (i + n - S (length ys)) by lia.
-        reflexivity.
-    - simplify decidable equality.
-      do 2 rewrite traverse_var.
-      simplify decidable equality.
-      replace (i + n - j) with i by lia.
-      destruct i; simpl.
-      + exfalso.
-        lia.
-      + replace (i - 0 + n - j) with i by lia.
-        replace (i - 0 + n - length ys) with (i + n - length ys) by lia.
-        reflexivity.
-    - now simplify decidable equality.
-  Qed.
+    admit.
+  Admitted.
+
+  (* New rule! Generalizes ShiftCons... *)
+  Lemma subst_ShiftApp:
+    forall i ys s,
+    i >= length ys ->
+    subst_comp (subst_lift i) (subst_app ys s) ~
+      subst_comp (subst_lift (i - length ys)) s.
+  Proof.
+    admit.
+  Admitted.
 
   (* IdL: I o s ~ s *)
   Lemma subst_IdL:
     forall s,
     subst_comp subst_ids s ~ s.
   Proof.
-    intros s k x.
-    unfold inst.
-    apply traverse_ext.
-    simpl; intros.
-    destruct (le_gt_dec j n).
-    - now rewrite traverse_var.
-    - now rewrite inst_fun_bvar.
-  Qed.
+    admit.
+  Admitted.
 
   (* IdR: s o I ~ s *)
   Lemma subst_IdR:
     forall s,
     subst_comp s subst_ids ~ s.
   Proof.
-    intros s k x.
-    unfold inst.
-    apply traverse_ext.
-    simpl; intros.
-    destruct (le_gt_dec j n).
-    - rewrite traverse_ext with (g := fun _ n => var n).
-      + now rewrite traverse_ids.
-      + intros i m ?.
-        now destruct (le_gt_dec i m).
-    - now rewrite inst_fun_bvar.
-  Qed.
+    admit.
+  Admitted.
 
   (* AssEnv: (s o t) o u ~ s o (t o u) *)
   Lemma subst_AssEnv:
     forall s t u,
     subst_comp (subst_comp s t) u ~ subst_comp s (subst_comp t u).
   Proof.
-    intros s t u k x.
-    unfold inst.
-    apply traverse_ext.
-    simpl; intros.
-    destruct (le_gt_dec j n).
-    - rewrite traverse_fun.
-      apply traverse_ext.
-      intros i m ?.
-      destruct (le_gt_dec i m).
-      + now replace (i + j - j) with i by lia.
-      + rewrite inst_fun_bvar by lia.
-        rewrite traverse_var.
-        now rewrite inst_fun_bvar by lia.
-    - reflexivity.
-  Qed.
+    admit.
+  Admitted.
 
   (* MapEnv: (y, s) o t ~ (y[t], s o t) *)
   Lemma subst_MapEnv:
@@ -905,44 +613,20 @@ Section DeBruijn.
     (* Note that we generalize this to the polyadic case! *)
     subst_comp (subst_app ys s) t ~ subst_app (smap t 0 ys) (subst_comp s t).
   Proof.
-    intros ys s t k x.
-    apply traverse_ext; simpl; intros.
-    destruct (le_gt_dec j n).
-    - admit.
-    - reflexivity.
+    admit.
   Admitted.
 
   (* SCons: (0[s], S o s) ~ s *)
   Lemma subst_SCons:
-    forall s k n m,
-    k = 0 ->
+    forall s n m,
     m = 1 + n ->
     (* We want to simplify a drop! Notice k has to be 0 to avoid lifting. *)
     (* TODO: I believe this can be generalized... do we want it? *)
-    subst_app [s k (var n)] (subst_comp (subst_lift m) s) ~
+    subst_app [inst s (var n)] (subst_comp (subst_lift m) s) ~
       subst_comp (subst_lift n) s.
   Proof.
-    intros s k n m ? ?; subst.
-    intros k x; unfold inst.
-    apply traverse_ext.
-    intros j m ?; simpl.
-    destruct (lt_eq_lt_dec j m) as [ [ ? | ? ] | ? ].
-    - simplify decidable equality.
-      remember (m - j) as o.
-      destruct o.
-      + exfalso.
-        lia.
-      + simpl.
-        destruct o; simpl; do 2 f_equal; lia.
-    - simplify decidable equality.
-      replace (traverse (inst_fun s)) with (inst s) by auto.
-      replace (m - j) with 0 by lia; simpl.
-      rewrite subst_lift_inst_commute by lia.
-      unfold lift; rewrite traverse_var.
-      unfold lift_fun; simpl.
-      do 2 f_equal; lia.
-    - now simplify decidable equality.
-  Qed.
+    admit.
+  Admitted.
 
   (* ShiftLift1: S o U(s) ~ s o S, variants A and B *)
   Lemma subst_ShiftLift1A:
@@ -951,23 +635,8 @@ Section DeBruijn.
     subst_comp (subst_lift i) (subst_upn j s) ~
       subst_comp (subst_lift (i - j)) (subst_comp s (subst_lift j)).
   Proof.
-    intros i j s ? k x.
-    unfold inst.
-    apply traverse_ext; simpl; intros l n ?.
-    destruct (le_gt_dec l n).
-    - fold (lift_fun j) (lift j).
-      do 2 rewrite traverse_var.
-      simplify decidable equality.
-      do 2 rewrite <- traverse_var.
-      fold (inst s).
-      rewrite subst_lift_inst_commute by lia.
-      f_equal.
-      unfold lift, lift_fun.
-      rewrite traverse_var.
-      simplify decidable equality.
-      f_equal; lia.
-    - reflexivity.
-  Qed.
+    admit.
+  Admitted.
 
   Lemma subst_ShiftLift1B:
     forall i j s,
@@ -975,23 +644,8 @@ Section DeBruijn.
     subst_comp (subst_lift i) (subst_upn j s) ~
       subst_comp (subst_upn (j - i) s) (subst_lift i).
   Proof.
-    intros i j s ? k x.
-    unfold inst.
-    apply traverse_ext; simpl; intros l n ?.
-    destruct (le_gt_dec l n).
-    - fold (lift_fun i) (lift i).
-      rewrite traverse_var.
-      simplify decidable equality.
-      do 2 rewrite <- traverse_var.
-      fold (inst s).
-      rewrite subst_lift_inst_commute by lia.
-      f_equal.
-      + lia.
-      + unfold lift, lift_fun.
-        rewrite traverse_var.
-        now simplify decidable equality.
-    - reflexivity.
-  Qed.
+    admit.
+  Admitted.
 
   (* ShiftLift2: S o (U(s) o t) ~ s o S o t, variants A and B *)
   Lemma subst_ShiftLift2A:
@@ -1001,29 +655,8 @@ Section DeBruijn.
       subst_comp (subst_lift (i - j)) (subst_comp s
         (subst_comp (subst_lift j) t)).
   Proof.
-    intros i j s ? k x.
-    unfold inst.
-    apply traverse_ext; simpl; intros l n ?.
-    destruct (le_gt_dec l n).
-    - do 2 rewrite traverse_var.
-      simplify decidable equality.
-      replace (i + n) with (j + (i - j + n)) by lia.
-      do 2 rewrite <- traverse_var.
-      fold (inst s).
-      rewrite <- baz by lia.
-      unfold inst; simpl.
-      do 2 rewrite traverse_fun.
-      do 2 rewrite traverse_var.
-      simplify decidable equality.
-      replace (l + l - l) with l by lia.
-      rewrite traverse_fun.
-      apply traverse_ext; intros p m ?.
-      destruct (le_gt_dec p m).
-      + f_equal; lia.
-      + rewrite traverse_var.
-        now rewrite inst_fun_bvar by lia.
-    - reflexivity.
-  Qed.
+    admit.
+  Admitted.
 
   Lemma subst_ShiftLift2B:
     forall i j s t,
@@ -1031,19 +664,7 @@ Section DeBruijn.
     subst_comp (subst_lift i) (subst_comp (subst_upn j s) t) ~
       subst_comp (subst_upn (j - i) s) (subst_comp (subst_lift i) t).
   Proof.
-    intros i j s t ? k x.
-    unfold inst.
-    apply traverse_ext; simpl; intros l n ?.
-    destruct (le_gt_dec l n).
-    - rewrite traverse_var.
-      simplify decidable equality.
-      destruct (le_gt_dec (j + l) (i + n)).
-      + admit.
-      + do 2 rewrite inst_fun_bvar by lia.
-        do 2 rewrite traverse_var.
-        simplify decidable equality.
-        now rewrite traverse_var.
-    - reflexivity.
+    admit.
   Admitted.
 
   (* Lift1: U(s) o U(t) ~ U(s o t), variants A and B *)
@@ -1053,22 +674,8 @@ Section DeBruijn.
     subst_comp (subst_upn k s) (subst_upn j t) ~
       subst_upn j (subst_comp (subst_upn (k - j) s) t).
   Proof.
-    intros s t k j ? l x.
-    unfold inst.
-    apply traverse_ext; simpl; intros p n ?.
-    destruct (le_gt_dec p n).
-    - destruct (le_gt_dec (j + p) n).
-      + replace (k - j + (j + p)) with (k + p) by lia.
-        fold (inst t).
-        rewrite <- subst_inst_lift.
-        (* Not easy to spot, but... *)
-        reflexivity.
-      + rewrite inst_fun_bvar by lia.
-        rewrite traverse_var.
-        simplify decidable equality.
-        now rewrite inst_fun_bvar by lia.
-    - reflexivity.
-  Qed.
+    admit.
+  Admitted.
 
   Lemma subst_Lift1B:
     forall s t k j,
@@ -1076,29 +683,8 @@ Section DeBruijn.
     subst_comp (subst_upn k s) (subst_upn j t) ~
       subst_upn k (subst_comp s (subst_upn (j - k) t)).
   Proof.
-    intros s t k j ? l x.
-    unfold inst.
-    apply traverse_ext; simpl; intros p n ?.
-    destruct (le_gt_dec p n).
-    - destruct (le_gt_dec (k + p) n).
-      + replace ((fun k0 n0 =>
-          if le_gt_dec k0 n0
-          then inst_fun t (j - k + k0) n0
-          else var n0)) with (inst_fun (subst_upn (j - k) t)) by auto.
-        fold (inst (subst_upn (j - k) t)).
-        rewrite <- subst_inst_lift.
-        unfold inst; simpl.
-        apply traverse_ext; intros q m ?.
-        destruct (le_gt_dec (k + q) m).
-        * simplify decidable equality.
-          f_equal; lia.
-        * now rewrite inst_fun_bvar by lia.
-      + rewrite inst_fun_bvar by lia.
-        rewrite traverse_var.
-        simplify decidable equality.
-        now rewrite inst_fun_bvar by lia.
-    - reflexivity.
-  Qed.
+    admit.
+  Admitted.
 
   (* Lift2: U(s) o (U(t) o u) ~ U(s o t) o u, variants A and B *)
   Lemma subst_Lift2A:
@@ -1127,42 +713,7 @@ Section DeBruijn.
     subst_comp (subst_upn n s) (subst_app (y :: ys) t) ~
       subst_app [y] (subst_comp (subst_upn (n - 1) s) (subst_app ys t)).
   Proof.
-    intros n s y ys t ? k x.
-    apply traverse_ext; intros j m ?.
-    simpl.
-    destruct (lt_eq_lt_dec j m) as [ [ ? | ? ] | ? ].
-    - simplify decidable equality.
-      destruct (le_gt_dec (n + j) m).
-      + replace (n + j) with (1 + (n - 1 + j)) by lia.
-        replace m with (1 + (m - 1)) at 1 by lia.
-        rewrite <- traverse_var.
-        fold (inst s).
-        rewrite <- baz by lia.
-        unfold inst.
-        rewrite traverse_var.
-        simpl.
-        simplify decidable equality.
-        rewrite traverse_fun.
-        remember (m - j) as o.
-        destruct o; try lia; simpl.
-        replace (nth_error [] o) with (@None X) by now destruct o.
-        (* I really need to rework those laws... *)
-        admit.
-      + do 2 rewrite inst_fun_bvar by lia.
-        do 2 rewrite traverse_var.
-        remember (m - j) as o.
-        destruct o; try lia; simpl.
-        replace (nth_error [] o) with (@None X) by now destruct o.
-        simplify decidable equality.
-        replace (m - 1 - j) with o by lia.
-        replace (m - 1 - length ys) with (m - S (length ys)) by lia.
-        reflexivity.
-    - simplify decidable equality.
-      rewrite inst_fun_bvar by lia.
-      rewrite traverse_var.
-      replace (m - j) with 0 by lia; simpl.
-      now simplify decidable equality.
-    - now simplify decidable equality.
+    admit.
   Admitted.
 
   (* New rule! Hmm... *)
@@ -1172,35 +723,17 @@ Section DeBruijn.
     subst_comp (subst_upn n s) (subst_app ys t) ~
       subst_app ys (subst_comp (subst_upn (n - length ys) s) t).
   Proof.
-    intros n s ys t ? k x.
-    apply traverse_ext; intros j m ?.
-    simpl.
-    destruct (le_gt_dec j m).
-    - (* I'm not sure why fold doesn't work in here, sorry. *)
-      replace (fun k n => ?[X]) with (inst_fun (subst_app ys t)) by auto.
-      (* Are we substituting something for a term in ys? *)
-      remember (m - j) as o.
-      remember (nth_error ys o) as y.
-      destruct y as [ y | ].
-      + (* We are; thus, the upn can't change the variable as the level is too
-           high, so we're only left to apply the app substitution. For starter,
-           we're out of reach for s. *)
-        assert (nth_error ys o <> None) by congruence.
-        apply nth_error_Some in H1.
-        rewrite inst_fun_bvar by lia.
-        (* This gotta return y to us. *)
-        rewrite traverse_var; simpl.
-        simplify decidable equality.
-        rewrite <- Heqo, <- Heqy.
-        reflexivity.
-      + (* We're above ys, so we will apply s, up to something, and then t. *)
-        assert (nth_error ys o = None) by congruence.
-        apply nth_error_None in H1.
-        simplify decidable equality.
-        replace (n - length ys + j) with (n + j - length ys) by lia.
-        fold (inst (subst_app ys t)) (inst t).
-        admit.
-    - reflexivity.
+    admit.
+  Admitted.
+
+  (* New rule! Hmm... *)
+  Lemma subst_LiftApp2:
+    forall n s ys zs t,
+    n >= length ys ->
+    subst_comp (subst_upn n s) (subst_app (ys ++ zs) t) ~
+      subst_app ys (subst_comp (subst_upn (n - length ys) s) (subst_app zs t)).
+  Proof.
+    admit.
   Admitted.
 
   (* LiftId: U(I) ~ I *)
@@ -1208,43 +741,24 @@ Section DeBruijn.
     forall i,
     subst_upn i subst_ids ~ subst_ids.
   Proof.
-    intros i k x.
-    unfold inst.
-    apply traverse_ext; simpl; intros.
-    destruct (le_gt_dec j n).
-    - now destruct (le_gt_dec (i + j) n).
-    - reflexivity.
-  Qed.
+    admit.
+  Admitted.
 
   (* ShiftShift (additional!): S^i o S^j = S^(i + j) *)
   Lemma subst_ShiftShift:
     forall i j,
     subst_comp (subst_lift i) (subst_lift j) ~ subst_lift (i + j).
   Proof.
-    intros i j k x.
-    unfold inst.
-    apply traverse_ext; simpl; intros l n ?.
-    destruct (le_gt_dec l n).
-    - rewrite traverse_var.
-      simplify decidable equality.
-      f_equal; lia.
-    - reflexivity.
-  Qed.
+    admit.
+  Admitted.
 
   (* LiftLift (additional!): U^i(U^j(s)) = U^(i+j)(s) *)
   Lemma subst_LiftLift:
     forall i j s,
     subst_upn i (subst_upn j s) ~ subst_upn (i + j) s.
   Proof.
-    intros i j s k x.
-    apply traverse_ext; simpl; intros l n ?.
-    destruct (le_gt_dec l n).
-    - destruct (le_gt_dec (i + l) n).
-      + f_equal; lia.
-      + destruct s; simpl;
-        now simplify decidable equality.
-    - reflexivity.
-  Qed.
+    admit.
+  Admitted.
 
   (* New rule! *)
   Lemma subst_AppNil:
@@ -1254,9 +768,21 @@ Section DeBruijn.
     admit.
   Admitted.
 
+  (* New rule! *)
+  Lemma subst_AppApp:
+    forall s xs ys,
+    subst_app xs (subst_app ys s) ~ subst_app (xs ++ ys) s.
+  Proof.
+    admit.
+  Admitted.
+
   (* ---------------------------------------------------------------------- *)
 
 End DeBruijn.
+
+(* *)
+
+Global Opaque lift subst inst_rec inst smap bsmap.
 
 (* *)
 
@@ -1268,7 +794,12 @@ Arguments subst_comp {X}.
 Arguments subst_upn {X}.
 Arguments subst_app {X}.
 
-(* Todo: we should move the notation to this place instead of copying it. *)
+(* *)
+
+(* TODO: turn this into a definition afterwards...? *)
+
+Global Notation subst_drop i :=
+  (subst_comp (subst_lift i)).
 
 Global Notation subst_cons y :=
   (subst_app [y]).
@@ -1282,11 +813,14 @@ Ltac sigma_solver :=
   | |- @deBruijnLaws _ _ =>
     typeclasses eauto
   | |- ?G =>
-    idtac "trying to solve" G;
+    (* idtac "trying to solve" G; *)
     (* TODO: rewrite those if they are within the context of a substitution;
        this can most certainly be done by using proper setoid rewriting. *)
-    repeat rewrite smap_length;
-    repeat rewrite bsmap_length;
+    try repeat (rewrite smap_length
+         || rewrite bsmap_length
+         || rewrite app_length
+         || rewrite last_length
+         || simpl length);
     lia
   end.
 
@@ -1295,11 +829,13 @@ Ltac sigma_solver :=
 Global Hint Rewrite subst_lift_unfold: sigma.
 Global Hint Rewrite subst_subst_unfold: sigma.
 
-Global Hint Rewrite subst_BVar using sigma_solver: sigma.
-Global Hint Rewrite subst_LiftInst using sigma_solver: sigma.
+(* Global Hint Rewrite subst_BVar using sigma_solver: sigma. *)
+(* Global Hint Rewrite subst_LiftInst using sigma_solver: sigma. *)
+Global Hint Rewrite subst_Inst using sigma_solver: sigma.
 Global Hint Rewrite subst_Id using sigma_solver: sigma.
 Global Hint Rewrite subst_FVarCons using sigma_solver: sigma.
 Global Hint Rewrite subst_RVarCons using sigma_solver: sigma.
+Global Hint Rewrite subst_VarApp using sigma_solver: sigma.
 Global Hint Rewrite subst_VarShift1 using sigma_solver: sigma.
 Global Hint Rewrite subst_VarShift2 using sigma_solver: sigma.
 Global Hint Rewrite subst_FVarLift1 using sigma_solver: sigma.
@@ -1308,13 +844,14 @@ Global Hint Rewrite subst_RVarLift1 using sigma_solver: sigma.
 Global Hint Rewrite subst_RVarLift2 using sigma_solver: sigma.
 Global Hint Rewrite subst_Clos using sigma_solver: sigma.
 (* -------------------------------------------------------------------------- *)
-Global Hint Rewrite baz using sigma_solver: sigma.
+(* Global Hint Rewrite baz using sigma_solver: sigma. *)
 (* -------------------------------------------------------------------------- *)
 
 Global Hint Rewrite subst_ShiftZero using sigma_solver: sigma.
 Global Hint Rewrite subst_LiftZero using sigma_solver: sigma.
 Global Hint Rewrite subst_VarShift using sigma_solver: sigma.
 Global Hint Rewrite subst_ShiftCons using sigma_solver: sigma.
+Global Hint Rewrite subst_ShiftApp using sigma_solver: sigma.
 Global Hint Rewrite subst_IdL using sigma_solver: sigma.
 Global Hint Rewrite subst_IdR using sigma_solver: sigma.
 Global Hint Rewrite subst_AssEnv using sigma_solver: sigma.
@@ -1330,19 +867,23 @@ Global Hint Rewrite subst_Lift2A using sigma_solver: sigma.
 Global Hint Rewrite subst_Lift2B using sigma_solver: sigma.
 Global Hint Rewrite subst_LiftEnv using sigma_solver: sigma.
 Global Hint Rewrite subst_LiftApp using sigma_solver: sigma.
+Global Hint Rewrite subst_LiftApp2 using sigma_solver: sigma.
 Global Hint Rewrite subst_LiftId using sigma_solver: sigma.
 Global Hint Rewrite subst_ShiftShift using sigma_solver: sigma.
 Global Hint Rewrite subst_LiftLift using sigma_solver: sigma.
 Global Hint Rewrite subst_AppNil using sigma_solver: sigma.
+Global Hint Rewrite subst_AppApp using sigma_solver: sigma.
 
 (* TODO: rewrite those only within the context of a substitution! *)
 
-Global Hint Rewrite smap_length: sigma.
-Global Hint Rewrite smap_nil: sigma.
-Global Hint Rewrite smap_cons: sigma.
-Global Hint Rewrite bsmap_length: sigma.
-Global Hint Rewrite bsmap_nil: sigma.
-Global Hint Rewrite bsmap_cons: sigma.
+Global Hint Rewrite smap_length using sigma_solver: sigma.
+Global Hint Rewrite smap_nil using sigma_solver: sigma.
+Global Hint Rewrite smap_cons using sigma_solver: sigma.
+Global Hint Rewrite smap_upn using sigma_solver: sigma.
+Global Hint Rewrite bsmap_length using sigma_solver: sigma.
+Global Hint Rewrite bsmap_nil using sigma_solver: sigma.
+Global Hint Rewrite bsmap_cons using sigma_solver: sigma.
+Global Hint Rewrite bsmap_upn using sigma_solver: sigma.
 
 (* TODO: figure out a way to restrict these rewritings. *)
 
@@ -1369,6 +910,7 @@ Ltac sigma :=
   (* TODO: is it possible to fold var in here...? *)
   (rewrite_strat topdown (hints sigma));
   (* TODO: we want to restrict the context in those... somehow... *)
+  simpl length;
   (rewrite_strat try topdown (hints sigma_cleanup)).
 
 (* -------------------------------------------------------------------------- *)
@@ -1422,16 +964,16 @@ Section Tests.
   Qed.
 
   Goal
-    forall x,
+    forall k x,
     (* Id: x[I] = x *)
-    subst_ids 0 x = x.
+    subst_ids k x = x.
   Proof.
     intros.
     now sigma.
   Qed.
 
   Goal
-    forall x s t,
+    forall s t x,
     (* Clos: x[s][t] = x[s o t] *)
     t 0 (s 0 x) = subst_comp s t 0 x.
   Proof.
@@ -1604,9 +1146,9 @@ Section Tests.
   Qed.
 
   Goal
-    forall k x,
+    forall i k x,
     (* LiftId: U(I) ~ I *)
-    subst_upn 1 subst_ids k x = subst_ids k x.
+    subst_upn i subst_ids k x = subst_ids k x.
   Proof.
     intros.
     now sigma.
@@ -1618,7 +1160,6 @@ Section Tests.
      lambda-calculus". *)
 
   Local Ltac equal_modulo_arith :=
-    (* TODO: do we want this to be global...? *)
     reflexivity || assumption || lia || (progress f_equal; equal_modulo_arith).
 
   Local Hint Extern 0 => equal_modulo_arith: core.
@@ -1636,7 +1177,17 @@ Section Tests.
     (* Instantiation and lifting commutation. *)
     forall x s i k j,
     k <= j ->
-    lift i k (inst s j x) = inst s (i + j) (lift i k x).
+    lift i k (s j x) = s (i + j) (lift i k x).
+  Proof.
+    intros.
+    now sigma.
+  Qed.
+
+  Goal
+    (* Instantiation and substitution commutation. *)
+    forall x y i k j,
+    k <= j ->
+    lift i k (subst y j x) = subst y (i + j) (lift i k x).
   Proof.
     intros.
     now sigma.
@@ -1699,22 +1250,27 @@ Section Tests.
     subst (var 1) n (lift (2 + n) 1 b).
   Proof.
     intros.
+    sigma.
+    replace (S (S n)) with (2 + n) by auto.
     (* This is not yet proved by sigma. TODO: figure out why! Nevertheless, a
-       simple check on n seems enough... *)
+       simple check on n seems almost enough... *)
     destruct n.
     - now sigma.
-    - sigma.
-      admit.
+    - admit.
   Admitted.
 
-  (* An useful, and true, property. This is required by the machine semantics,
-     and, indeed, sigma is able to solve it. *)
+  (* An useful property. This is required by the machine semantics; luckly, we
+     can solve it using sigma with a very simple case analysis. *)
   Goal
     forall s p k n,
     s (p + k) (var (p + n)) = lift p 0 (s k (var n)).
   Proof.
     intros.
-    now sigma.
+    destruct (le_gt_dec k n).
+    - now sigma.
+    - now sigma.
   Qed.
+
+  (* TODO: can we make right_cycle_right_cycle_simplification simpler? *)
 
 End Tests.
